Support for Coq 8.20 (#115)
* port to Coq 8.20

* fix ml

* strings

* fix CI

* use Equations 1.3.1.

* fix benchmarks

* fix bootstrap

* disable trace printing

theories/LambdaBoxMut/compile.v
@@ -340,6 +340,7 @@ Fixpoint list_Defs (l : list (def Term)) : Defs :=
 Polymorphic Equations trans_prim_val {T} (p : EPrimitive.prim_val T) : option primitive :=
   trans_prim_val (existT _ primInt (primIntModel i)) => Some (existT _ AstCommon.primInt i) ;
   trans_prim_val (existT _ primFloat (primFloatModel i)) => Some (existT _ AstCommon.primFloat i) ;
+  trans_prim_val (existT _ primString _) => None ;
   trans_prim_val (existT _ primArray _) => None.
 
 Section LiftSize.
