cplugin/PrimString.v
@@ -1,0 +1,10 @@
+From CertiCoq.VanillaPlugin Require Import Loader.
+From Coq Require Import PString.
+
+CertiCoq Register [
+  Coq.Strings.PrimString.compare => "prim_string_compare",
+  Coq.Strings.PrimString.get => "prim_string_get",
+  Coq.Strings.PrimString.length => "prim_string_length"
+]
+Include [ Library "prim_string.h" ].
+
